lib/pipeline.ml
@@ -1,4 +1,4 @@
-open Moore0
+open Moore1
 open Alphabet
 open Teacher
 open Dfa
@@ -89,14 +89,8 @@ module DFAPipeline
     (Tch : DFATEACHER with module S = S)
     (L : DFALEARNER) =
 struct
-  module Compiler = DFACompiler (S) (Tch.D)
+  module Compiler = DFACompiler (S) (Tch.D) (Moore.Moore (S) (Out))
   module Lrn = L (Tch)
-
-  let moore_of_dfa (d : 'a Tch.D.t) : 'a Compiler.Moore.t =
-    { Compiler.Moore.transition= d.Tch.D.transition
-    ; Compiler.Moore.initial= d.Tch.D.initial
-    ; Compiler.Moore.output= d.Tch.D.accept
-    ; Compiler.Moore.states= d.Tch.D.states }
 
   let learned : Obj.t Tch.D.t option ref = ref None
 
@@ -136,7 +130,7 @@ struct
       (unit, string) Stdlib.result =
     let d = learn () in
     name_idents base ;
-    match Compiler.compile_program (moore_of_dfa d) eq_dec base with
+    match Compiler.compile_dfa d eq_dec base with
     | Error e ->
         Stdlib.Error ("Error: " ^ e)
     | Ok p ->
@@ -202,7 +196,7 @@ module NFAPipeline
     (Tch : NFATEACHER with module S = S)
     (L : NFALEARNER) =
 struct
-  module Compiler = NFACompiler (S) (Tch.R.N)
+  module Compiler = NFACompiler (S) (Tch.R.N) (DFA.DFA (S)) (Moore.Moore (S) (Out))
   module Lrn = L (Tch)
 
   let learned : Obj.t Tch.R.t option ref = ref None
@@ -229,7 +223,7 @@ struct
     reg 2 "table" ;
     reg 3 "init" ;
     reg 4 "final" ;
-    reg 17 "run"
+    reg 10 "run"
 
   (** Compile the learned NFA to Clight and print it to [output_fn] or [stdout]
 
